definitions/ident.v
@@ -1,0 +1,118 @@
+Require Import FSets.FMaps.
+Require Structures.OrderedType.
+Require Import Nat.
+Require Import Arith.PeanoNat.
+Require Import Arith.Bool_nat.
+Require Import String.
+
+Require Import ssreflect ssrfun ssrbool.
+
+Module Type IDENTfun (Map : S).
+
+  Notation t := Map.key.
+
+  Parameter new : forall elt : Type, Map.t elt -> t.
+
+  Axiom new_spec :
+      forall elt : Type, forall s : Map.t elt,
+      ~ Map.In (new elt s) s.
+      
+End IDENTfun.
+
+Module Type IDENT.
+
+  Declare Module Map : S.
+
+  Include IDENTfun Map. 
+
+End IDENT.
+
+Module IdentFacts (Import Ident : IDENT).
+
+  Module OTFacts := OrderedTypeFacts Map.E.
+
+  Notation eq := Map.E.eq.
+
+  Notation eqb := OTFacts.eqb.
+
+  Lemma eqb_spec :
+      forall x y : t, Bool.reflect (eq x y) (eqb x y).
+  Proof.
+    intros x y.
+    apply Bool.iff_reflect.
+    unfold eqb.
+    destruct OTFacts.eq_dec;
+    constructor;
+    auto.
+    intro Heq.
+    discriminate Heq. 
+  Qed.
+
+End IdentFacts.
+
+Module NatMap := FMapList.Make (Structures.OrderedTypeEx.Nat_as_OT).
+
+Module NatIdent <: IDENT.
+
+  Module Map := NatMap.
+  
+  Definition eqb := Nat.eqb.
+
+  Infix "=?" := eqb (at level 70).
+
+  Definition max {elt} (s : NatMap.t elt) :=
+    NatMap.fold (fun x _ acc => Nat.max x acc) s O.
+  
+  Definition new {elt} (s : NatMap.t elt) :=
+    S (max s).
+
+  Lemma max_geq {elt} (s : NatMap.t elt) (x : nat) :
+      NatMap.In x s -> max s >= x.
+  Proof.
+    intro Hin.
+    destruct Hin as [e Hmap].
+    unfold max.
+    rewrite NatMap.fold_1.
+    apply NatMap.elements_1 in Hmap.
+    generalize O.
+    induction Hmap; intro n.
+    - destruct H as [Heq _].
+      unfold NatMap.E.eq in Heq.
+      simpl in Heq.
+      simpl.
+      rewrite Heq.
+      eapply PeanoNat.Nat.le_trans.
+    --- exact (PeanoNat.Nat.le_max_l y.1 n).
+    --- generalize (Nat.max y.1 n).
+        clear n.
+        induction l;
+        simpl;
+        intro n.
+    ----- apply PeanoNat.Nat.le_refl.
+    ----- eapply PeanoNat.Nat.le_trans.
+    ------- exact (PeanoNat.Nat.le_max_r a.1 n).
+    ------- exact (IHl (Nat.max a.1 n)).
+    - simpl.
+      exact (IHHmap (Nat.max y.1 n)).
+  Qed.
+
+  Lemma new_spec {elt} (s : NatMap.t elt) :
+      ~ NatMap.In (new s) s.
+  Proof.
+    unfold new.
+    intro HIn.
+    have : (S (max s)) <= max s.
+    - exact (max_geq s (S (max s)) HIn).
+    - intro Hleq.
+      rewrite <- Nat.lt_succ_r in Hleq.
+      exact (Nat.lt_irrefl _ Hleq).
+  Qed.
+
+End NatIdent.
+
+
+
+
+
+
+
