definitions/types.v
@@ -1,9 +1,33 @@
 Declare Scope system_t_type_scope.
 
+Require Import Nat.
+Require Import ident.
+
+Declare Module TIdent : IDENT.
+
+Module TIdentFacts := IdentFacts TIdent.
+
+Infix "=?t" := TIdentFacts.eqb (at level 70).
+
+Definition tident := TIdent.t.
+
 Inductive typeT :=
   | natT : typeT
   | boolT : typeT
-  | tT : nat -> typeT
+  | tvarT : tident -> typeT
   | funT : typeT -> typeT -> typeT.
 
 Notation "t ->T u" := (funT t u) (at level 80, right associativity).
+
+Fixpoint tvarT_subst (x : tident) (t a : typeT) :=
+  match t with
+  | tvarT y =>
+    match x =?t y with
+    | true => a
+    | _ => tvarT y
+    end
+  | funT t u =>
+    funT (tvarT_subst x t a) (tvarT_subst x u a)
+  | t =>
+    t
+  end.
