definitions/typing.v
@@ -1,26 +1,62 @@
 Require Import types.
 Require Import terms.
 Require Import FSets.FMaps.
+Require Import List.
 
 Open Scope system_t_type_scope.
 Open Scope system_t_term_scope.
 
-Module FMap := FMapPositive.PositiveMap.
+Module FMap := FIdent.Map.
 
-Definition context := FMap.t typeT.
+Record context := {
+  bmap : list typeT;
+  fmap : FMap.t typeT
+}.
 
-Print context.
+Definition bpush (t : typeT) (G : context) := {|
+  bmap := t :: (bmap G);
+  fmap := fmap G
+|}.
 
-(* Inductive typing_derivation : context -> termT -> typeT -> Type :=
-  | var :
-    forall G, forall n, forall t, G n = Some t ->
-    TypingDerivation G (xT n) t
-  | oTnatT :
-    forall G, TypingDerivation G oT natT
-  | sTnatT :
-    forall G, forall e, TypingDerivation G e natT ->
-    TypingDerivation G (sT e) natT. 
-*)
+Inductive typing_derivation : context -> termT -> typeT -> Type :=
+  | bvarT_ax :
+    forall G : context, forall n : nat, forall t : typeT,
+    nth_error (bmap G) n = Some t ->
+    typing_derivation G (bvarT n) t
+  | fvarT_ax :
+    forall G : context, forall x : fident, forall t : typeT,
+    FMap.MapsTo x t (fmap G) ->
+    typing_derivation G (fvarT x) t
+  | absT_in :
+    forall G : context, forall e : termT, forall t u : typeT,
+    typing_derivation (bpush t G) e u ->
+    typing_derivation G (absT e) (t ->T u)
+  | appT_el :
+    forall G : context, forall e f : termT, forall t u : typeT,
+    typing_derivation G e (t ->T u) ->
+    typing_derivation G f t ->
+    typing_derivation G (appT e f) u
+  | trueT_ax :
+    forall G : context, typing_derivation G trueT boolT
+  | falseT_ax :
+    forall G : context, typing_derivation G falseT boolT
+  | iteT_el :
+    forall G : context, forall e f g : termT, forall t : typeT,
+    typing_derivation G e boolT ->
+    typing_derivation G f t ->
+    typing_derivation G g t ->
+    typing_derivation G (iteT e f g) t
+  | oT_ax :
+    forall G : context, typing_derivation G oT natT
+  | sT_el :
+    forall G : context, forall e : termT, typing_derivation G e natT ->
+    typing_derivation G (sT e) natT
+  | recT_el :
+    forall G : context, forall e f g : termT, forall t : typeT,
+    typing_derivation G e t ->
+    typing_derivation G f (t ->T natT ->T t) ->
+    typing_derivation G g natT ->
+    typing_derivation G (recT e f g) t.
 
 Close Scope system_t_type_scope.
 Close Scope system_t_term_scope.
